add unfold hints, parser equivalence example

deps/poulet4/examples/IntExample.v
@@ -29,7 +29,7 @@ Definition EmptyParser : Declaration tag_t := DeclConstant tag_t tag constTyp na
 (* Let's just parse an int... *)
 
 (* 
-parser IntExample (packet_in pkt, out int output) {
+parser IntExample (packet_in pkt, out int<2> output) {
   state start {
     pkt.extract(output);
     transition accept;
@@ -38,17 +38,15 @@ parser IntExample (packet_in pkt, out int output) {
 *)
 
 Definition scope : Env_EvalEnv := MkEnv_EvalEnv nil nil "dummy".
-(* Definition good_scope : Env_EvalEnv := MkEnv_EvalEnv  *)
 
 Definition pkt_param : P4Parameter := MkParameter true Directionless (TypExtern "packet_in") "pkt".
 Definition out_type : P4Type := TypInt 2.
 Definition out_param : P4Parameter := MkParameter true Out out_type "output".
 Definition locals : list (Declaration tag_t) := nil.
-Definition accept_st : ParserState tag_t := MkParserState _ tt (MkP4String _ tt String.accept) nil (ParserDirect _ tt (MkP4String _ tt String.accept)).
 Definition output_expr : Expression tag_t := MkExpression _ tt (ExpName _ (BareName "output")) out_type Directionless.
-Definition pkt_extract_expr : Expression tag_t := MkExpression _ tt (ExpName _ (BareName "pkt")) (TypFunction (MkFunctionType nil ((MkParameter false Directionless out_type "x")::nil) FunBuiltin out_type)) Directionless.
-Definition extract_stmt : Statement tag_t := 
-  MkStatement _ tt (StatMethodCall _ (MkExpression _ tt (ExpExpressionMember _ pkt_extract_expr (MkP4String _ tt String.extract)) TypVoid Directionless) (out_type :: nil) (Some output_expr :: nil)) StmVoid.
+Definition pkt_extract_expr : Expression tag_t := MkExpression _ tt (ExpName _ (BareName "pkt")) (TypFunction (MkFunctionType nil ((MkParameter false Directionless out_type "t")::nil) FunBuiltin out_type)) Directionless.
+Definition build_extract_stmt (into_type: P4Type) (into_expr: Expression tag_t) := MkStatement _ tt (StatMethodCall _ (MkExpression _ tt (ExpExpressionMember _ pkt_extract_expr (MkP4String _ tt String.extract)) TypVoid Directionless) (into_type :: nil) (Some into_expr :: nil)) StmVoid.
+Definition extract_stmt : Statement tag_t := build_extract_stmt out_type output_expr.
 
 
 Definition body: list (Statement tag_t) := extract_stmt :: nil.
@@ -114,153 +112,182 @@ Proof.
   unfold states.
   unfold start_st.
   unfold parses.
-  unfold step_trans. auto.
+  unfold step_trans. simpl.
   unfold run_with_state.
-  unfold good_env.
-  unfold Monad.mbind.
-  unfold state_monad_inst.
-  unfold state_bind.
+  unfold good_env. auto.
 
-  unfold step.
-  unfold lookup_state.
+  unfold state_bind. simpl.
+
+  unfold eval_statement. simpl.
+  
+  unfold state_bind. simpl.
+  unfold Environment.toss_value. simpl.
+
+  unfold eval_method_call. simpl.
+  unfold state_bind. simpl.
+  unfold Environment.find_environment, Environment.push_scope. simpl.
+  unfold Environment.lift_env_lookup_fn, Environment.find_environment'.
   simpl.
-  unfold Monad.mbind. unfold state_monad_inst. unfold state_bind.
-  unfold body. 
+  rewrite top_find_pkt. simpl.
 
-  unfold eval_statement.
-  unfold Monad.mbind. unfold state_monad_inst. unfold state_bind.
-  unfold Environment.map_env. unfold Environment.push_scope. unfold Environment.extend_scope.
-  auto.
-  unfold Monad.mret. unfold state_monad_inst. unfold state_return.
+  unfold eval_builtin_func. simpl.
+  unfold state_bind. simpl.
 
-  unfold states_to_block. unfold List.fold_right.
-  unfold extract_stmt.
-
-  unfold eval_method_call.
-  unfold eval_expression. unfold pkt_extract_expr.
-  unfold Environment.find_environment. unfold Environment.lift_env_lookup_fn.
-  unfold Monad.mbind. unfold state_monad_inst. unfold state_bind.
-  unfold Environment.toss_value.
-  unfold Environment.find_environment'.
-  unfold Environment.str_of_name_warning_not_safe.
-  auto.
-
-
-  assert (H := top_find_pkt).
-  unfold Environment.MStr.find. unfold Environment.MStr.Raw.find. auto.
-  unfold Environment.MStr.this. 
-  unfold Environment.MStr.empty. unfold Environment.MStr.Raw.empty.
-
+  unfold Environment.find_environment, Environment.lift_env_lookup_fn, Environment.find_environment'. simpl.
+  rewrite top_find_val. simpl.
+  unfold Environment.dummy_value, eval_packet_func. simpl.
+  unfold state_bind. simpl.
+  unfold Environment.find_lvalue. simpl.
+  unfold Environment.lift_env_lookup_fn, Environment.find_environment'. simpl.
+  rewrite top_find_pkt. simpl.
+  unfold Environment.update_lvalue. simpl.
+  unfold Environment.lift_env_fn, Environment.update_environment'. simpl.
   
   
-  unfold Environment.MStr.find in H. unfold Environment.MStr.Raw.find in H. 
-
-  unfold Environment.MStr.this in H.
-  rewrite H.
-  clear H.
-
-  unfold Monad.mret. unfold state_monad_inst. unfold state_return.
-  unfold pkt_value.
-  unfold String.extract.
-
-  simpl.
-  unfold extract_value_func. unfold eval_builtin_func.
-
-  unfold Monad.mbind. unfold state_monad_inst. unfold state_bind.
-  unfold eval_arguments.
-  unfold Monad.mbind. unfold state_monad_inst. unfold state_bind.
-  unfold eval_expression. unfold output_expr.
-
-  unfold Environment.find_environment. unfold Environment.lift_env_lookup_fn. unfold Environment.find_lvalue'.
-  unfold Environment.find_environment'. unfold Environment.str_of_name_warning_not_safe.
+  unfold Option.option_bind.
   
-  unfold Environment.MStr.find. unfold Environment.MStr.Raw.find. auto.
+  rewrite top_find_pkt. simpl.
+  unfold Environment.insert_scope. simpl.
+  unfold Option.option_bind. rewrite top_find_pkt. simpl.
 
-  unfold Environment.MStr.this.
-  assert (H := top_find_val).
-
-  unfold Environment.MStr.find in H. unfold Environment.MStr.Raw.find in H. auto.
-
-  unfold Environment.MStr.this in H.
-  rewrite H. clear H.
-
-  unfold Monad.mret. unfold state_monad_inst. unfold state_return.
-
-  unfold String.extract. 
-  unfold String.isValid.
-  unfold String.setValid.
-  unfold String.setInvalid.
-  unfold String.pop_front. simpl.
-  unfold String.push_front. simpl.
-  unfold is_packet_func.
-  unfold String.extract. 
-
-  unfold Environment.dummy_value.
-  unfold eval_packet_func.
-  unfold Monad.mbind. unfold state_monad_inst. unfold state_bind.
-  unfold Environment.find_lvalue. unfold Environment.lift_env_lookup_fn. unfold Environment.find_lvalue'.
-  unfold Environment.find_environment'. unfold Environment.str_of_name_warning_not_safe.
-  unfold Environment.MStr.this.
-  unfold Environment.MStr.find. unfold Environment.MStr.Raw.find. auto.
-
-  unfold Environment.MStr.this.
-
-  assert (H := top_find_pkt).
-  unfold Environment.MStr.find in H. unfold Environment.MStr.Raw.find in H.
-  unfold Environment.MStr.this in H.
-  rewrite H. clear H.
-
-  unfold Monad.mret. unfold state_monad_inst. unfold state_return.
-
-  unfold pkt_value.
-  unfold String.extract. simpl in *.
-  unfold Packet.eval_packet_extract_fixed.
-  unfold out_type.
-
-  unfold Monad.mbind. unfold state_monad_inst. unfold state_bind.
-  unfold Packet.read_first_bits.
-  unfold Monad.mret. unfold state_monad_inst. unfold state_return.
-
-
-  unfold Environment.update_lvalue. unfold Environment.lift_env_fn. unfold Environment.update_lvalue'.
-  
-  unfold Environment.update_environment'.
-  unfold Environment.str_of_name_warning_not_safe.
-  unfold Environment.MStr.find. unfold Environment.MStr.Raw.find. unfold Environment.MStr.this.
-
-
-  unfold Monad.mbind. unfold state_monad_inst. unfold state_bind.
-
-  assert (H := top_find_pkt).
-  unfold Environment.MStr.find in H. unfold Environment.MStr.Raw.find in H.
-  unfold Environment.MStr.this in H.
-  rewrite H. clear H.
-  unfold Option.option_monad_inst. unfold Option.option_bind.
-  (* unfold Environment.update_scope. *)
-  unfold Environment.insert_scope.
-
-  unfold Monad.mbind. unfold Option.option_monad_inst. unfold Option.option_bind.
-
-  rewrite top_find_pkt.
-
-  unfold Monad.mret. unfold Option.option_ret. unfold state_return.
-
-  unfold eval_lvalue.
-  unfold Monad.mret. unfold state_monad_inst. unfold state_return.
-
-  assert (H := top_find_val_inter).
-  unfold Environment.MStr.find in H. unfold Environment.MStr.Raw.find in H. unfold Environment.MStr.this in H.
-  unfold inter_scope in H.
-  rewrite H. clear H.
-  assert (H := top_find_val_inter).
-  unfold inter_scope in H.
-  rewrite H. clear H.
-
-  unfold Environment.pop_scope.
-  unfold eval_transition.
-  unfold Monad.mret. unfold state_monad_inst. unfold state_return.
-  unfold String.accept. 
-  simpl.
-  auto.
+  fold inter_scope. rewrite top_find_val_inter. 
+  now simpl.
 Qed.
+
+
+(* OK, now consider the following two parsers: *)
+(* 
+parser Tupled (packet_in pkt, out int x, out int y) {
+  state start {
+    pkt.extract(x);
+    pkt.extract(y);
+    transition accept;
+  }
+}
+
+parser Curried (packet_in pkt, out int x, out int y) {
+  state start {
+    pkt.extract(x);
+    transition middle;
+  }
+  state middle {
+    pkt.extract(y);
+    transition accept;
+  }
+}
+
+An interesting property is that Tupled and Curried behave the same on all packets!
+*)
+
+Definition x_param : P4Parameter := MkParameter true Out out_type "x".
+Definition y_param : P4Parameter := MkParameter true Out out_type "y".
+Definition x_expr : Expression tag_t := MkExpression _ tt (ExpName _ (BareName "x")) out_type Directionless.
+Definition y_expr : Expression tag_t := MkExpression _ tt (ExpName _ (BareName "y")) out_type Directionless.
+Definition extract_x := build_extract_stmt out_type x_expr.
+Definition extract_y := build_extract_stmt out_type y_expr.
+
+Definition body_tupled := extract_x :: extract_y :: nil.
+Definition body_1_curried := extract_x :: nil.
+Definition body_2_curried := extract_y :: nil.
+
+Definition start_st_tupled : ParserState tag_t := MkParserState _ tt (MkP4String _ tt "start") body_tupled (ParserDirect _ tt (MkP4String _ tt String.accept)).
+Definition start_st_curried : ParserState tag_t := MkParserState _ tt (MkP4String _ tt "start") body_1_curried (ParserDirect _ tt (MkP4String _ tt "middle")).
+Definition mid_st_curried : ParserState tag_t := MkParserState _ tt (MkP4String _ tt "middle") body_2_curried (ParserDirect _ tt (MkP4String _ tt String.accept)).
+
+Definition states_tupled : list (ParserState tag_t) := start_st_tupled :: nil.
+Definition states_curried : list (ParserState tag_t) := start_st_curried :: nil.
+
+Definition IntParserTupled := ValObjParser _ scope nil nil states_tupled.
+Definition IntParserCurried := ValObjParser _ scope nil nil states_curried.
+
+Definition build_env (bits: list bool): Environment.environment tag_t := 
+  Environment.extend_scope _ "pkt" (ValObj _ (ValObjPacket _ bits)) (
+    Environment.extend_scope _ "x" out_value (
+      Environment.extend_scope _ "y" out_value (
+        Environment.MStr.empty _
+      )
+    )
+  ) :: nil.
+
+Lemma find_x : 
+  forall bits: list bool,
+  Environment.find_scope _ "x" (List.hd (Environment.MStr.empty _) (build_env bits)) = Some out_value.
+Proof.
+Admitted.
+
+Lemma curried_tupled_equiv: 
+  forall (bits: list bool),
+    parses IntParserTupled 4 "start" (build_env bits) = parses IntParserCurried 4 "start" (build_env bits).
+Proof.
+  (* induction bits.
+  unfold build_env, IntParserTupled, IntParserCurried, parses. simpl.
+  unfold run_with_state. simpl.
+  unfold state_bind. simpl.
+  unfold eval_statement. simpl.
+  unfold state_bind. simpl.
+  unfold Environment.toss_value. simpl.
+  unfold eval_method_call. simpl.
+  unfold state_bind. simpl.
+
+  unfold Environment.find_environment, Environment.lift_env_lookup_fn, Environment.find_environment'.
+  simpl.
+  unfold Environment.extend_scope. simpl. 
+  
+  assert (lookup_env := Environment.MStr.find_1).
+  specialize (lookup_env (Value tag_t)).
+  remember (
+  (Environment.MStr.add "x" out_value
+     (Environment.MStr.add "y" out_value
+        (Environment.MStr.empty (Value tag_t))))) as env_inner.
+  remember (Environment.MStr.add "pkt" (ValObj tag_t (ValObjPacket tag_t nil)) env_inner) as env.
+  specialize (lookup_env env).
+
+  pose proof (lookup_env "pkt") as lookup_pkt.
+
+  rewrite Heqenv in lookup_pkt.
+
+  pose proof (@Environment.MStr.add_1 (Value tag_t) env_inner "pkt" "pkt") as add_pkt.
+  specialize (add_pkt (ValObj tag_t (ValObjPacket tag_t nil))).
+
+  assert (pkt_eq := eq_refl "pkt").
+  specialize (add_pkt pkt_eq).
+
+  specialize (lookup_pkt (ValObj tag_t (ValObjPacket tag_t nil)) add_pkt).
+
+  rewrite <- Heqenv in lookup_pkt.
+  rewrite lookup_pkt. simpl.
+
+  unfold eval_builtin_func. simpl.
+  unfold state_bind. simpl.
+  
+
+  unfold Environment.push_scope. simpl.
+
+  assert (Fx := find_x).
+
+  unfold build_env in Fx.
+
+  unfold Environment.find_environment, Environment.lift_env_lookup_fn, Environment.find_environment'.
+  simpl.
+
+  pose proof (lookup_env "x") as lookup_x.
+
+  (* rewrite Heqenv in lookup_x. *)
+
+  pose proof (@Environment.MStr.add_1 (Value tag_t) env_inner "x" "x") as add_x.
+  specialize (add_pkt (ValObj tag_t (ValObjPacket tag_t nil))).
+
+  unfold Environment.MStr.find, Environment.MStr.Raw.find. simpl.
+  rewrite Heqenv.
+  rewrite Heqenv_inner.
+  unfold Environment.MStr.Raw.add. simpl.
+  unfold Environment.MStr.Raw.add. simpl.
+  unfold String.ascii_compare. simpl.
+  unfold Bool.reflect_dec. auto.
+  unfold BinNat.N.ltb_spec0. simpl.
+  unfold and_rec. simpl.
+  (* cbv beta. cbv delta. *)
+  simpl.
+  unfold env. *)
+Admitted.
 
